# Monday February 17th

Last time:
The second character formula (equation (2)),

\begin{align*}
ch L(\lambda) =  \ch M(\lambda) + \sum_{\mu < \lambda, \mu \in W\cdot \lambda} b_{\lambda, \mu} \ch M(\mu)
.\end{align*}

Note that $b_{\lambda, \mu} \in \ZZ$, and this formula comes from inverting the previous one.

> Holy grail: characters of simple modules!

We can write $M(\lambda) \cong U(\lien^-) \tensor_\CC \CC_\lambda$ as a $\lieh\dash$module.
Define $p: \lieh\dual \to \ZZ$ where $p(\gamma)$ is the number of tuples $(t_\beta)_{\beta\in\Phi^+}$ where $t_\beta \in \ZZ^+$ and $\gamma = - \sum_{\beta \in \Phi^+} t_\beta \beta$.
We have $\supp p = - \ZZ^+ \Phi^+$, which gives us something like a negative quadrant of the lattice.
The function $p$ is essentially the *Kostant partition function*. 
The advantage here is that $p \in \mcx$ (defined last time, support is less than some finite weights?).

*Observation:*
$p = \ch_{M(0)}$ since $U(\lien^-) \tensor \CC_{\lambda = 0}$ has PBW basis $\theset{ \prod_{\beta\in\Phi^+} y_\beta^{t_\beta} \tensor 1_{\lambda = 0} \suchthat t_\beta \in \ZZ^+  }$.


*Example:* 
Let $\lieg = \liesl(3)$, then $\Phi^+ = \theset{\alpha_1, \alpha_2, \alpha_1 + \alpha_2}$.
Then $\gamma = -\qty{\alpha_1 + 2\alpha_2}$ corresponds to $(1,2,0), (0,1,1)$ so $p(\gamma) = 2$.
If $\gamma = -\qty{2\alpha_1 + 2\alpha_2}$, this corresponds to $(2,2,0), (1,1,1), (0,0,2)$ so $p(\gamma) = 3$.

> Note: just the number of ways of obtaining $-\gamma$ as a linear combinations of roots.

In general, $\dim M(0)_\gamma = p(\gamma)$.

**Proposition:**
For any $\lambda \in \lieh\dual$, we have $\ch_{M_\lambda} = p\ast e_\gamma$, taking the convolution product.
In particular, $\ch_{M(0)} = p$.

*Proof:*

\begin{align*}
(p\ast e_\lambda)(\lambda+\gamma) 
&= p(\gamma) e_\lambda(\lambda) \\
&= p(\gamma) 1 \\ 
&= p(\gamma) \\
&= \dim M(\lambda)_{\lambda + \gamma} \quad\text{ as a weight space }
.\end{align*}

$\qed$

Note that we can also write equation (2) as

\begin{align*}
\ch L(\lambda) = \sum_{w\cdot \lambda \leq \lambda} b_{\lambda, w} \ch M(w\cdot \lambda)
.\end{align*}

Here $b_{\lambda, w} \in \ZZ$ and in fact $b_{\lambda, 1} = 1$.

*Example:*
Let $\lieg = \liesl(2)$.
We know

\begin{align*}
\ch M(\lambda) &= \ch L(\lambda) + \ch L(s_\alpha \cdot \lambda) \\
ch M(s_\alpha \cdot \lambda) &= \ch L(s_\alpha \cdot \lambda)
.\end{align*}

We can think of this pictorially as the 'head' on top of the socle:

\begin{align*}
M(\lambda) = \frac{L(\lambda)}{L(s_\alpha \cdot \lambda)}
.\end{align*}

The formula above corresponds to the matrix
$
\left[\begin{array}{cc} 1 & 1 \\ 0 & 1 \end{array}\right]
$

We can invert the formula to get equation (2), which corresponds to inverting this matrix:

\begin{align*}
\ch L(\lambda) &= \ch M(\lambda) - \ch M(s_\alpha \cdot \lambda) \\
\ch L(s_\alpha \cdot \lambda) &= \ch M(s_\alpha \cdot \lambda)
.\end{align*}

Note that the coefficients $b_{w, \lambda} \in \theset{0, \pm 1}$ in this equation are independent of $\lambda \in \Lambda^+$.

If $\lambda \not\in\Lambda^+$, then $\ch L(\lambda) = \ch M(\lambda)$ and $b_{\lambda, 1} = 1, b_{\lambda, s_\alpha} = 0$ are again independent of $\lambda \in \lieh\dual \setminus \Lambda^+$.

**Question:**
To what extent to $b_{\lambda, w}$ depend on $\lambda$?
The answer is seemingly "not much".

## 

> Note: skipping chapter 2 since we're focusing on infinite dimensional representations.
