# Fall 2015

1. Lemma: $f$ is injective $iff f$ has a left inverse $f\inv$ satisfying $f\inv f(a) = a$.
   
   Suppose $f,g: A \to A$ are injective and $x,y \in A$, we want to show that $(f\circ g)(x) = (f\circ g)(y) \implies x = y$. So suppose $f(g(x)) = f(g(y))$. Since $f$ is injective, $f$ has a left inverse, so $g(x) = g(y)$, and since $g$ is injective $x = y$. $\qed$

2. Claim: take $\delta < \min(1, \sqrt{\frac{\varepsilon}{5}})$. Then $\abs{x-2} < \delta \implies 1 < x < 2 \implies 1 > \frac 1 x > \frac 1 2$, so in particular $\frac 1 x < 1$ and
   $$\begin{align*}
   \abs{x + \frac 1 x - \frac 5 2} &= \abs{\frac{2x^2 - 5x + 2}{2x}}\\
   &< \frac 1 2 \abs{(2x^2-4x + 2) - x}\\
   &= \frac 1 2 \abs{2(x-2)^2 + 3(x-2)} \\
   &< \abs{2(x-2)^2 + 3(x-2)} \\
   &\leq 2\abs{x-2}^2 + 3\abs{x-2} \\
   &< 2\delta^2 + 3\delta \\ 
   &< 5\delta^2  \hspace{10em} \text{since } \delta < 1 \implies \delta^2 < \delta \\
   &< 5 \left(\sqrt{\frac{\varepsilon}{5}}\right)^2 \\
   &= \varepsilon.
   \end{align*}$$
   $\qed$

1. Denoting $D^n f \definedas \dd{^n f}{x^n}$ and noting that $D^1 D^n f = D^{n+1}f$, we have
  $$\begin{align*}
  D^0f &= xe^{2x} \\
  D^1f &= e^{2x} + 2D^0f \\
  D^2f &= 2e^{2x} + 2D^1f \\
  D^3f &= 4e^{2x} + 2D^2f \\
  \end{align*}$$

    and (claim) so we find that 
  $$D^n f = 2^{n-1}e^{2x} + 2D^{n-1}f.$$
  
    This is trivially the case for $n=1$, where we've computed $D^1 f = e^2x + 2xe^{2x} = 2^0e^{2x} + 2D^0 f$, and the inductive step holds exactly because 
  $$
  D^{n+1}f = DD^{n}f \\
  = D(2^{n-1}e^{2x} + 2D^{n-1}f) \\
  =2^n e^{2x} + 2D^n f.
  $$
  $\qed$

1. It will exactly be the row space of $$A = \left(\begin{array}{rrrr}
1 & 1 & 1 & 1 \\
3 & 4 & 6 & 7 \\
5 & 6 & 8 & 9
\end{array}\right)$$, where we could note that $R_3 = 2R_1 + R_2$ but $R_1 \neq \lambda R_2$ and so the first two rows span the correct subspace. We can also easily compute the RREF, which has the same rowspace, $$\tilde A = \left(\begin{array}{rrrr}
1 & 0 & -2 & -3 \\
0 & 1 & 3 & 4 \\
0 & 0 & 0 & 0
\end{array}\right)$$
from which we find that $\vector v_1 = \thevector{1,0,-2,-3}$ and $\vector v_2 = \thevector{0,1,3,4}$ also do the job. $\qed$

1. We have $p_A(x) = (x+1)(x-1)(x) = x^3 - x$ and so by Cayley-Hamilton, $A^3 - A = 0 \implies A^3 = A$. $\qed$

1. We first need the derivatives of $\arctan$, since
    $$
    T(p, x) = \sum_{n=0}^\infty \frac{f^{(n)}(p)}{n!}(x-p)^n \implies T(0, x) = \sum_{n=0}^\infty \frac{f^{(n)}(0)}{n!}x^n 
    $$

    Starting with $y=\arctan x$, we can write $\tan y - x = 0 \implies \sec^2y~dy - 1~dx = 0$ by implicit differentiation and the chain rule,and so $\dd{y}{x} = y' = \sec^{-2}y = \cos^2(\arctan x))$. Embed this in a triangle with angle $y$ to find that $y' = (1+x^2)^{-1}$.

    Computing many derivatives of this directly is tedious, so instead we'll take a power series: 
    $$
    (1+x^2)\inv = \sum_{n=0}^\infty (-x^2)^n \\
    = \sum_{n=0} (-1)^{n}x^{2n}\\
    =1 - x^2 + x^4 - x^6 + x^8 - x^{10} + \cdots \\
    \implies \dd{}{x} (1+x^2)\inv = -2x + 4x^3 - 6x^5 \\
    = \sum_{n=1}^\infty (2n)(-1)^{n}x^{2n-1}\\
    \implies \dd{^m}{x^m} (1+x^2)\inv = \sum_{n=m}^\infty(2n)(2n-1)\cdots(2n-m+1)(-1)^nx^{2n-m}\\
    \implies \restrictionof{ \dd{^m}{x^m} (1+x^2)\inv}{x = 0} = \frac{(2m)!}{m!}
    $$ 

    since only the constant term survives. Thus the $n$ coefficient of the Taylor expansion about zero will be 
    $$
    T_{2m} = \frac{(2m!)}{m!m!} = {2m \choose m}
    $$