# Fall 2017 

1. 
   1. Negate $\forall x\in \RR,~\exists y\in \RR \suchthat \abs{x-y} \geq 2017$
   $$\exists x\in \RR \suchthat \forall y\in \RR,~ \abs{x-y} < 2017$$

   1. Note that $p\implies q \iff q \vee \neg p$, so we have $\neg(p \implies q) \iff \neg(q \vee \neg p) \iff p ~\&~ \neg q$.
$$
f: \RR \to \RR \text{ is continuous } \iff \\ 
\forall (x, y) \in \RR^2, ~\forall \varepsilon,~\exists \delta \suchthat \quad d(x,y) < \delta \implies d(f(x), f(y)) < \varepsilon \iff \\ 
\forall (x, y) \in \RR^2, ~\forall \varepsilon,~\exists \delta \suchthat \quad  d(x,y) \geq \delta ~~\vee~~   d(f(x), f(y)) < \varepsilon  ,
$$
so
$$
f: \RR \to \RR \text{ is not continuous } \iff \\ \exists (x,y) \in \RR^2, \exists \varepsilon \suchthat \forall \delta, \quad d(x,y) < \delta ~\&~ d(f(x), f(y)) \geq \varepsilon. \qed
$$

1. $V = \theset{\vector v \in \RR^3 \suchthat \inner{\vector v}{\thevector{3,4,5}} = \vector 0}$
   1. Subspace test: $V \subset X$ is a linear subspace iff $\theset{t\vector v_1 + \vector v_2 \suchthat t\in \RR, \vector v_i \in V} \subseteq V$.
   $$
   \inner{t\vector v_1 + \vector v_2}{\thevector{3,4,5}} = t\inner{\vector v_1}{\thevector{3,4,5}} + \inner{\vector v_2}{\thevector{3,4,5}} = t\vector 0 + \vector 0 = \vector 0.\qed
   $$
      1. Alternatively, just note that it is the kernel of the linear map $\inner{\wait}{\thevector{3,4,5}}: \RR^3 \to \RR^1$, and kernels are always sub-things.
   1. Note $V$ defines a plane $P \cong \RR^2 \subset \RR^3$, so a projection onto $P^\perp = \thevector{3,4,5}$ will work:
   $$
   A = \left[ \begin{array}{ccc} 3 & 4 & 5 \\ 0 & 0 & 0 \\ 0 & 0 & 0\end{array}\right]
   $$
   Then $A\vector x = \thevector{3x + 4y + 5z, 0, 0}$ and if $\vector x \in V$ then this is zero by definition of $V$.
   1. Yes, get two vectors in the plane using the "nullspace" trick, then take the orthogonal projection $A(A^TA)\inv A^T$
   2. No, by rank nullity: $\abs{\im A} + \abs{\ker A} = \abs{\mathrm{domain} A}$.
   
2. Induct on $n$, integrate by parts and use L'Hopital.

3. 
   1. Cayley-Hamilton
   2. 
   $$
   \left(\begin{array}{rr|r}
      1 & 1 & 0 \\
      0 & 1 & 0 \\
      \hline
      0 & 0 & -1
      \end{array}\right),~ A^2 = \left(\begin{array}{rrr}
        1 & 2 & 0 \\
        0 & 1 & 0 \\
        0 & 0 & 1
        \end{array}\right), \quad
      \spec(A) = [-1, 1, 1]
   $$
   1. Every symmetric matrix with real spectrum can be diagonalized over $\RR$ by the spectral theorem, so $A$ is similar to a diagonal matrix $D$ with the same eigenvalues ($\pm 1$). But $D^2_{ii} = (\pm 1)^2$ so $D^2 = I$. 

4. 
   - Definition of uniform convergence:
  $$
  \theset{f_n}_{i=1}^\infty\rightrightarrows f \text{ on } X  \iff \forall \varepsilon > 0,~ \exists N(\varepsilon) \suchthat n\geq N(\varepsilon) \implies \forall x \in X,~ \abs{f_n(x) - f(x)} < \varepsilon
  $$
    - **Theorem** (Riemann-Lebesgue): A bounded function on a compact set is integrable iff its set of discontinuities has measure zero.

    - **Theorem**: 
  $$
  f_n \rightrightarrows f \implies \lim_{n\to\infty} \int_X f_n(x) ~dx = \int_X  \lim_{n\to\infty} f_n(x) ~dx = \int_X f(x) ~dx
  $$
    - *Proof* (Pugh 218): 
    
      - Fix $f_n$; by the Riemann-Lebesgue theorem $f_n$ is bounded, and discontinuous only at finitely many points $Z_n$, and thus bounded and continuous on $[a,b] - Z_n$ where $\mu(Z_n) = 0$. A uniform limit of continuous functions is continuous, so $f$ is also continuous on $S = [a,b] - \union_n Z_n$. Thus $f$ is also bounded on $S_n$. A countable union of countable/measure zero sets is also countable/measure zero, so $f$ is bounded and discontinuous only on a countable set of measure zero, so $f$ is integrable. 
  
      - Finally, let $C_b(X, \RR) = \theset{f:X \to \RR \suchthat f\text{ is bounded }}$, which is a complete normed space under the norm $\norm{f}_\sup = \sup_{x\in X}\theset{\abs{f(x)}}$ which induces the metric 
      $$d(f,g) = \norm{f-g}_\sup = \sup_{x\in X}\theset{\abs{f(x) - g(x)}}.$$

      - Thus $f_n \rightrightarrows f \iff \norm{f-f_n}_\sup \to 0$, so we have
      $$\begin{align*}
      \abs{\int_a^b f(x)~dx - \int_a^b f_n(x)~dx} 
      &= \abs{\int_a^b f(x) - f_n(x)~dx} \\
      &\leq \int_a^b \abs{f(x) - f_n(x)}~dx \\
      &\leq \norm{f-f_n}_\sup \abs{b-a} \\
      & \to 0 \abs{b-a} = 0. \qed
      \end{align*}$$

1. Let $\delta = \min\theset{2, \sqrt\varepsilon}$, then 
$$\abs{x-1} < 2 \implies -2 < x-1 < 2 \implies -1 < x < 3 \implies \abs{x} < 3 \implies \frac 1 {\abs x} < \frac 1 3$$ and so
  $$\begin{align*}
  \abs{x-1} < \delta \implies \abs{\frac{x^2+1}{x} - 2} 
  &= \abs{\frac{(x-1)^2}{x}} \\
  &= \frac{\abs{x-1}^2}{\abs{x}} \\
  &< \frac{\varepsilon}{\abs{x}} \\
  &< \frac{\varepsilon}{3} \\
  &< \varepsilon. \qed
  \end{align*}$$

1. Definitions:
  - $f: \RR^2 \to \RR, \quad (x,y) \mapsto z = f(x,y)$
  - Level curves are given by $f(x, y) = c$; 
  - $\nabla f: \RR^2 \to \RR^2, \quad \nabla f(\vector p) = \thevector{f_x(\vector p), f_y(\vector p)}$
  - $\gamma(t): \RR \to \RR^2, \quad \gamma(t) = \thevector{x(t), y(t)}, \quad \gamma_t(t) = \thevector{x_t(t), y_t(t)}$
  - $g(t) = f \circ \gamma:\RR \to \RR, \quad (f \circ \gamma)(t) = f(x(t), y(t)), \quad g_t(t) = f_t(\gamma(t))\cdot \gamma_t(t)$
  - A vector $v$ is perpendicular to a surface at a point $p$ iff $v$ is perpendicular to the tangent vector of every curve passing through $p$.
  - Proof of actual statement
    - Let $\vector p = \thevector{x_0, y_0}$ be a point on the level surface, so $f(\vector p) = c$ for some constant.
    - Let $\gamma(t) = \thevector{x(t), y(t)}$ be a curve on the level surface, so $\gamma(t_0) = \vector p$ for some $t_0$. 
    - Let $g(t) = f(x(t), y(t)) = (f \circ \gamma)(t)$, and note that $g(t_0) = f(\vector x) = c$ (for some $\vector x$) and so $g_t(t) = 0$.
    - By the chain rule, compute 
    $$\begin{align*}
    g_t(t) 
    &= (\dd{f}{x}\dd{x}{t} + \dd{f}{y}\dd{y}{t})(t) \\
    &= \inner{ \thevector{f_x(x(t), y(t)), f_y(x(t), y(t))} } { \thevector{x_y(t), y_t(t)} } \\ 
    &= \inner{\nabla f(\gamma(t))}{\gamma_t(t)}.
    \end{align*}$$ 

    Note that we have 
    $$ 
    g_t(t_0) =  \inner{\nabla f(\gamma(t_0))}{\gamma_t(t_0)} = \inner{\nabla f(\vector p)}{\gamma_t(t_0)}
    $$
    but by the previous statement, $g_t(t_0) = 0$, which exacty says that the gradient of $f$ is orthogonal to every $\gamma$ on the level surface, and thus orthogonal to the surface itself. $\qed$

1. Parts:
   1. Suppose $\forall x, g(f(x)) = x$. We want to show $f(a) = f(b) \implies a = b$. So let $a,b \in \mathrm{domain}(f)$, and suppose $f(a) = f(b)$. By assumption, we have $g(f(a)) = a$ and $g(f(b)) = b$, but then $f(a) = f(b) \implies g(f(a)) = g(f(b))$ and so $a = g(f(a)) = g(f(b)) = b$.
   2. Suppose $\forall x, g(f(x)) = x$. We want to show $\forall y \in \mathrm{codomain}(g), \exists x \in \mathrm{domain}(g) = \mathrm{codomain}(f)$ such that $f(x) = y$. Let $y$ \in \mathrm{codomain}(g) be arbitrary. Since here we also have $\mathrm{codomain}(g) = \mathrm{domain}(f)$, we can consider $f(y)$. By assumption, $g(f(\wait)) = \wait$ for all $\wait$, so let $x = f(y)$. Then $g(x) = y$ as desired. 
   3. Need to have $f$ fail surjectivity and $g$ fail injectivity, so take $X = [2],~ Y = [3]$, and 
   $$
   f(1) = 1, ~f(2) = 2\\ 
   g(1) = 1, ~g(2) = 2, ~g(3) = 2
   $$
   then $f((g(1)) = f(1) = 1, ~f(g(2)) = 2$, and this exhausts $X$. Since $X,Y$ are different sizes, this isn't a bijection -- in particular, $3\not\in\im f$.




