# Friday January 17th

Reference:
See Lang's Complex Analysis, there are plenty of solution manuals.

Let $f; \Omega \to \CC$ be a complex-valued function.
Recall that $f$ is *complex differentiable* iff the usual ratio/limit exists.
Note that $h = x+iy$ and $h\to 0 \iff x,y\to 0$.

We can write $f'(z) = \dd{f}{x} = \frac 1 i \dd{f}{y}$.
This follows from Cauchy-Riemann since $u_x = v_y$ and $u_y = -v_x$.

Definition:
We want to define $\del, \bar \del$ operators.
We have the identities

\begin{align*}
x = \frac{z + \bar z}{z} \quad y = \frac{z - \bar z}{iz}
.\end{align*}

We can then write

\begin{align*}
dz = dx + idy \\
d\bar z = dx - i dy
.\end{align*}


We define the dual operators by $\inner{\dd{}{z}}{dz} = 1$ and similarly $\inner{ \dd{}{\bar z}  }{d\bar z} = 1$.
By the chain rule, we can write

\begin{align*}
f_z &= f_x x_z + f_y y_z \\
&= \frac 1 2 f_x + f_y \frac{1}{2i} \\
&= \frac 1 2 \qty{\dd{}{x} + i \dd{}{y} }f 
,\end{align*}

and similarly $f_{\bar z} = f_x x_{\bar z} + f_y z_{\bar z} = \frac 1 2 \qty{ \dd{}{x} - \frac{1}{2i} \dd{}{y}  }f$.

We thus find $\del_x = \del_z + \del_{\bar z}$ and $\del_y = i\qty{ \del_z - \del_{\bar z}  }$,
and define

\begin{align*}
\del f &= \dd{f}{z} dz \\
\bar{\del} f &= \dd{f}{\bar z} d\bar z \\
df = f_z dz + f_{\bar z} d\bar z
.\end{align*}

Proposition:
$f$ is holomorphic iff $f_{\bar z} = 0$.

> This means that $f$ depends on $z$ alone and not $\bar z$.

Proof:
$\bar \del f = 0$ iff $\frac 1 2 (f_x + if_y) = 0$, so $(u_x  - v_y) + i (v_x + u_y) = 0$.
$\qed$

Application to PDEs:
We can write $u_{xx} = v_{xy}, u_{yy} = v_{yx}$ and so $u_{xx} + u_{yy} = 0 = v_{xx} + v_{yy}$.
Thus $\Delta f = 0$, and $f$ satisfies Laplace's equation and is said to be *harmonic*.

Corollary:
If $f$ is analytic, then $u, v$ are both harmonic functions.

**Theorem (Chain Rule):**
Let $w = f(z)$ and $g(w) = g(f(z))$.
Then

\begin{align*}
h_z &= g_w f_z + g_{\bar w} \bar f_z \\
h_{\bar z} &= g_w f_{\bar z} + g_{\bar w} \bar f_{\bar z}
.\end{align*}

If $f, g$ are holomorphic, $f_{\bar z} = g_{\bar w} = 0$, so $h_{\bar z} = 0$ and $h$ is holomorphic and $h_z = g_w f_z$.

Example:
Given a power series $f=\sum a_n (z- z_0)^n$.
Then

1. There exists a radius of convergence $R$ such that $f$ converges precisely on $D_R(z_0)$.
2. $f$ is continuous on $D_R(z_0)^\circ$.
3. By the root test, $R = (\limsup \abs{a_n}^{1/n})\inv = \liminf \abs{a_n/a_{n+1}} = (\limsup \abs{a_{k+1}/a_k})\inv$.

Recall the ratio test: $\sum a_k$ converges absolutely iff $\limsup \abs{a_{k+1} / a_k} < 1$

Theorem:
If $f(z) = \sum_{n=0} a_n z^n$ is holomorphic on $\abs{z} < R$ for $R> 0$ then $f'(z) = \sum_{n=1} a_n n z^{n-1}$.

This follows from the fact that $n^{\frac 1 n} \to 1$.
Also tricky: show $\lim \sin(n)$ doesn't exist.
