# Monday January 27th

Fix a connected domain $\Omega$ which is bounded with a piecewise $C^1$ boundary. 

**Theorem (Green's):**
Given $f, g \in C^1 \bar \Omega$, we can take a vector field $F = \generators{f, g}$ and have

\begin{align*}
\int_{\bd \Omega} f~dx + g~dy &= \iint_{\Omega} \qty{ \dd{g}{x} - \dd{f}{y}  } ~dA \\
\int_{\bd \Omega} - f~dx + g~dy &= \iint_{\Omega} \qty{ \dd{g}{x} + \dd{f}{y}  } ~dA \\
\int_{\bd \Omega} f~dy - g~dy &= \iint_{\Omega} \qty{ \dd{f}{x} + \dd{g}{y}  } ~dA \\
\int_{\bd \Omega} F \cdot \vector n ~ds &= \iint_{\Omega} \nabla \cdot F ~dA
\int_{\bd \Omega} \mathrm{curl}(F) ~ds &= \iint_{\Omega} \mathrm{div}(F) ~dA
,\end{align*}

where we take $\vector n$ to be orthogonal to $\bd \Omega$.
The quantities appearing on the RHS are referred to as the flux.

For $f(z) \in C^1(\Omega)$ holomorphic, we can then write

\begin{align*}
\int_{\bd \Omega} f ~dz
&= \int_{\bd \Omega} f ~(dx + idy) \\
&= \int_{\bd \Omega} f ~dx + if~dy \\
&= \iint_\Omega \qty{if_x - f_y} ~dA
&= 0
,\end{align*}

which follows since $f$ holomorphic, we can write $f'(z) = f_x = \frac 1 i f_y$, so $i f_x = f_y$ and thus $\dd{f}{\bar z} = 0$.

> See Taylor's Introduction to Complex Analysis

**Theorem (Cauchy's Integral Formula):**
If $f\in C^1(\bar \Omega)$ and $f$ is holomorphic, then for any $z\in \Omega$

\begin{align*}
f(z) = \frac{1}{2\pi i} \int_{\bd \Omega} \frac{d(\xi)}{\xi - z} ~d\xi
.\end{align*}

*Proof:*
Since $z\in \Omega$ an open set, we can find some $r> 0$ such that $D_r(z) \subset \Omega$.
Then $\frac{f(\xi)}{\xi - z}$ is holomorphic on $\Omega\setminus D_r(z)$.
Let $C_r = \bd D_r(z)$.

Claim 1:
$\int_{\bd \Omega} \frac{f(\xi)}{\xi - z} ~d\xi = \int_{C_r} \frac{f(\xi)}{\xi - z} ~ d\xi$.

Proof:
Use the parameterization of $C_r$ given by $\xi = z + re^{i\theta}$.
Then

\begin{align*}
\frac {1}{2\pi i} \int_{C_r} \frac{f(\xi)}{\xi - z} ~d\xi 
&= \frac {1}{2\pi i} \int_0^{2\pi} \frac{f(z + re^{i\theta})}{re^{i\theta}} ~ird\theta \\
&= \frac{1}{2\pi} \int_0^{2\pi} f(z + re^{i\theta}) ~d\theta \\
\converges{r\to 0} \frac{1}{2\pi} \int_{\bd \Omega} \frac{f(\xi)}{\xi - z}
.\end{align*}

where we use the fact that $f(z + re^{i\theta}) = f(z) + f'(z)re^{i\theta} + o(r) \to f(z)$.

Letting $F(\xi) = f(\xi)/(\xi - z)$, this is holomorphic on $\Omega\setminus D_r(z)$.
Let $\Omega_r = \bd \Omega \union (-C_r)$.
Take the following path integral:


![Image](figures/2020-01-27-13:59.png)

Then
\begin{align*}
0 = \int_{\bd \Omega_r} F(\xi) ~d\xi = \int_{\bd \Omega} F(\xi) ~d\xi - \int_{C_r} F(\xi) ~d\xi
,\end{align*}

which forces these integrals to be equal.

$\qed$

If we can differentiate through the integral, we can obtain

\begin{align*}
\dd{}{z} f(z) = \frac 1 {2\pi i} \int_{\bd \Omega} \frac{f(\xi)}{(\xi - z)^2} ~d\xi
.\end{align*}

and thus inductively

\begin{align*}
(D_z)^n f(z) = \frac{n!}{2\pi i} \int_{\bd \Omega} \frac{ f(\xi) ~d\xi  }{ (\xi - z)^{n+1}  }
.\end{align*}

To prove rigorously, need to write

\begin{align*}
\Delta_h f(z) 
= \frac 1 h \qty{ f(z+h) - f(z) } \\
= \frac 1 {2\pi i h} \int_{\bd \Omega} f(\xi) \qty{ \frac{1}{\xi - (z+h)} - \frac{1}{\xi - z}  } ~d\xi
= \frac 1 {2\pi i h} \int_{\bd \Omega} f(\xi) \qty{ \frac{1}{ (\xi - z- h)(\xi - z)  }  } ~d\xi
,\end{align*}

and show the integrand converges uniformly, where $\frac{1}{(\xi - z - h)(\xi - z)} \converges{u} \frac{1}{(\xi - z)^2}$.

Continuing inductively yields the integral formula. 

**Corollary:**
If $f$ is holomorphic, then $f\in C^1(\Omega)$ implies that $f \in C^\infty(\Omega)$.

Theorem: 
If $f$ is holomorphic in $\Omega$, then $f$ is equal to its Taylor series (i.e. $f(z_0$ is analytic.)

Fix $z_0 \in \Omega$ and let $r = \abs{z- z_0}$.

\begin{align*}
\frac{1}{\xi - z} 
&= \frac{1}{ \xi - z_0 - (z-z_0)  } \\
&= \frac{1}{\xi - z_0} \frac{1}{1 - \qty{ \frac{z-z_0}{\xi - z_0}   }  } \\
&= \frac{1}{\xi - z_0} \sum_n \qty{ \frac{z - z_0}{\xi - z_0}  }^n \quad\text{for } \abs{z - z_0} < \abs{\xi - z_0}
.\end{align*}

Note that $\sum z^n$ converges uniformly for any $\abs{z} < \delta < 1$.

Thus

\begin{align*}
f(z) 
&= \frac{1}{2\pi i} \int_{\xi \in \bd\Omega} f(\xi) \sum \frac{(z-z_0)^n}{(\xi - z_0)^{n+1}} ~d\xi \\
&= \sum \qty{ \frac {1}{2\pi i} \int \frac{f(\xi)  }{(\xi - z_0)^{n+1}} ~d\xi} (z-z_0)^n \\
&= \sum \frac{f^{(n)} (z_0)}{n!} (z-z_0)^n
.\end{align*}

$\qed$

Thus $f$ is holomorphic iff $f$ is analytic.


