# Wednesday February 26th

## Argument Principle and Application

Let $f$ be holomorphic in $\Omega$ which is open, simple, and connected.
Then $f(z_0) = 0$ implies there exists an integer $m$ such that $f(z) = (z-z_0)^m g(z)$ where $g(z_0) \neq 0$.

Let $N_\Omega(f)$ be the number of zeros of $f$ inside $\Omega$, and $N_\Omega(f, a)$ be the number of zeros of $f-a$ in $\Omega$.
Writing $f = f_1 f_2$ where $f_1 = (z-z_0)^m$ and $f_2 = g(z)$, we have

\begin{align*}
\frac f' f 
&= \frac f_1' f_1 + \frac f_2' f_2 \\
&= \frac m {z-z_0} + \frac g' g
.\end{align*}

Now integrating both sides yields

\begin{align*}
\frac 1 {2\pi i } \int_{D_r(z_0)} \frac{f'(z)}{f(z)} ~dz = m 
,\end{align*}

so the integral of this function counts the number of zeros of $f$ in $D_r(z_0)$.

Proposition (Argument Principle)
: Let $f$ be holomorphic in a neighborhood of $\bar{D_r(z_0)}$ and suppose that $f$ is non-vanishing on all of $\bd D_r(z_0)$.
  Then

  \begin{align*}
  \frac 1 {2\pi i } \int_{D_r(z_0)} \frac{f'(z)}{f(z)} ~dz = N_{D_r(z_0)}(f)
  .\end{align*}

  More generally, if $q(z)$ is another holomorphic function in a neighborhood of $\bar{D_r(z_0)}$ and $z_1, \cdots, z_k$ are the distinct zeros of $f$ in $D_r(z_0)$ with orders $m_1, \cdots, m_k$, then

  \begin{align*}
  \frac 1 {2\pi i } \int_{D_r(z_0)} q(z) \frac{f'(z)}{f(z)} ~dz
  = \sum_{j=1}^k q(z_k) m_k
  .\end{align*}

Proof
: Write $f(z) = \prod_{j=1}^k (z-z_j)^{m_j} g(z)$. 
  By Leibniz's rule, if $h = f_1 \cdots f_\ell$, then

  \begin{align*}
  \frac h' h 
  &= \sum_{j=1}^\ell \frac f_j' f_j \\
  \implies q\frac f' f = 1\frac g' g + \sum_{j=1}^k \frac{m_j q}{z-z_j}
  .\end{align*}

  Since $\frac g' g$ is holomorphic in the closed disc, integrating both sides yields the desired formula.

Note that if we replace $f$ by a family $f_t$ of continuous functions, an integer-valued continuous function must be constant.

Corollary
: Let $f_t(z)$ for $0\leq t \leq 1$ be a family of holomorphic functions on $D_{r+\eps}(z_0)$ for some $\eps > 0$.)
  Suppose $f_t(z)$ is continuous for all $z$ in this disc, uniformly in $z$, and for all $t$, $f_t(z)$ is nonvanishing on the boundary.
  
  Then the following integral is independent of $t$:

  \begin{align*}
    \frac 1 {2\pi i } \int_{D_r(z_0)} \frac{f_t'(z)}{f_t(z)} ~dz
  .\end{align*}

Theorem (Rouch√©'s)
: Let $f, g$ be holomorphic in a neighborhood of $\bar{D_r(z_0)}$ and suppose that on $\bd D_r(z_0)$ we have
  $$
  \abs{f(z) - g(z)} < \abs{f(z)} + \abs{g(z)}
  \label{star}
  $$
  Then $f$ and $g$ are nonvanishing on $\bd D_r(z_0)$ and

  \begin{equation}
  N_{D_r(z_0)} (f) =
  N_{D_r(z_0)} (g)
  .\end{equation}

Proof
:  If $f(w) = 0$ for some $w\in \bd D_r(z_0)$, then $\abs{-g(w)} = \abs{g(w)}$, but this contradicts condition \ref{star}.

  So let $t\in [0, 1]$ with $f_t(z) = (1-t)f(z) + t g(z)$.
  Then (claim) $f_t$ is nonvanishing on the boundary, so we can apply the previous corollary.
  
  Suppose otherwise that there exists $w$ on the boundary such that $f_t(w) = 0$ for some $t$, so $(1-t)f(w) + tg(w) = 0$.
  Then rearranging terms yields

  \begin{align*}
  f(w) &= t(g(w) - f(w)) \\
  g(w) &= (1-t)(g(w) - f(w))
  .\end{align*}

  But then

  \begin{align*}
  \abs{f(w) + g(w)} 
  &= t\abs{g(w) - f(w)} + (1-t) \abs{g(w) - f(w)} \\
  &= \abs{g(w) - f(w)}
  ,\end{align*}
  which contradicts condition \ref{star}

  By the corollary, the integral is continuous in $t$


