---
title: 8.8 Part 2, Computing the Index of $L$
---

What we're trying to prove:

- 8.1.5: $(d\mcf)_u$ is a Fredholm operator of index $\mu(x) - \mu(y)$.

- Define
\begin{align*}
L: W^{1, p}\left(\mathbb{R} \times S^{1} ; \mathbb{R}^{2 n}\right) & \longrightarrow L^{p}\left(\mathbb{R} \times S^{1} ; \mathbb{R}^{2 n}\right) \\
Y & \longmapsto \frac{\partial Y}{\partial s}+J_{0} \frac{\partial Y}{\partial t}+S(s, t) Y
\end{align*}
where 
\begin{align*}
S: \RR\cross S^1 &\to \mat(2n; \RR) \\
S(s, t) &\converges{s\to\pm\infty}\to S^\pm(t)
.\end{align*}

- 8.7: Shows $L$ is Fredholm

- By the end of 8.8: replace $L$ by $L_1$ with the same *index* 
  - *(not the same kernel/cokernel)*
- Compute $\ind L_1$: explicitly describe $\ker L_1, \coker L_1$. 

- Replace in two steps:
  - $L \leadsto L_0$, modified outside $B_{\sigma_0}(0)$ in $s$. 
    - Replace $S(s, t)$ by a matrix 
    \begin{align*}
    \tilde S(s, t) = 
    \begin{cases}
    S^-(t)   & s\leq -\sigma_0 \\
    S^+(t)   & s\geq \sigma_0 \\
    \end{cases}
    .\end{align*}
    - Idea: approximate by cylinders at infinity.
    - Use invariance of index under small perturbations.
  - $L_0 \leadsto L_1$ by a homotopy, where $S_\lambda: S \leadsto S(s)$ a diagonal matrix that is a constant matrix *outside* $B_\eps(0)$.
    - Use invariance of index under homotopy.

## Main Results

- Theorem 8.8.1:  
  \begin{align*}
  \ind(L) = \mu\left(R^{-}(t)\right)-\mu\left(R^{+}(t)\right)=\mu(x)-\mu(y)
  .\end{align*}

- Prop 8.8.2: Reducing $L$ to $L_1$ 
  Construct an operator
  \begin{align*}
  L_{1}: W^{1, p}\left(\mathbb{R} \times S^{1} ; \mathbb{R}^{2 n}\right) & \longrightarrow L^{p}\left(\mathbb{R} \times S^{1} ; \mathbb{R}^{2 n}\right) \\
  Y & \longmapsto \frac{\partial Y}{\partial s}+J_{0} \frac{\partial Y}{\partial t}+S(s) Y
  \end{align*}
  where $S: \RR \to\mat(2n; \RR)$ is a path of diagonal matrices depending on $\ind(R^\pm(t))$; then 
  $$\ind(L) = \ind(L_1) = \ind(R^-(t)) - \ind (R^+(t)).$$

- Prop 8.8.3: Reducing $L_1$ to $R^\pm$.
  Let $k^\pm \definedas \ind(R^\pm)$; then $\ind(L_1) = k^- - k^+$.

- Lemma 8.8.4: $\ind(L_0) = \ind(L)$.

- Han's Talk:
  - Prop 8.8.3, using Lemma 8.8.5
- Me
  - Proof of 8.8.5

## 8.8.5: 


Used in the proof of 8.8.3, $\ind(L_1) = K^- - k^+$.

Setup:
\begin{align*}
S(s)=\left(\begin{array}{cc}
a_{1}(s) & 0 \\
0 & a_{2}(s)
\end{array}\right), \quad \text { with } a_{i}(s)=\left\{\begin{array}{ll}
a_{i}^{-} & \text {if } s \leq-s_{0} \\
a_{i}^{+} & \text {if } s \geq s_{0}
\end{array}\right.
.\end{align*}


Statement: let $p>2$ and define
\begin{align*}
F: W^{1, p}\left(\mathbb{R} \times S^{1} ; \mathbb{R}^{2}\right) &\longrightarrow L^{p}\left(\mathbb{R} \times S^{1} ; \mathbb{R}^{2}\right) \\
Y &\mapsto \frac{\partial Y}{\partial s}+J_{0} \frac{\partial Y}{\partial t}+S(s) Y
.\end{align*}

> This looks like $L_1$ for $n=1$?

1.  Suppose $a_1(s) = a_2(s)$ and define $a^\pm \definedas a_1^\pm = a_2^\pm$.
    Then
    \begin{align*}
      \operatorname{dim} \operatorname{Ker} F &=
      2 \cdot \#\left\{\ell \in \mathbf{Z} | a^{-} < 2 \pi \ell < a^{+}\right \} \\
      \operatorname{dim} \operatorname{Ker} F^{\star} &=
      2 \cdot \#\left\{\ell \in \mathbf{Z} | a^{+}<2 \pi \ell<a^{-}\right\}
    .\end{align*}

2.  Suppose $\sup_{s\in \RR} \norm{S(s)} < 1$, then
    \begin{align*}
    \operatorname{dim} \operatorname{Ker} F &= 
    \#\left\{i \in\{1,2\} \suchthat ~a_{i}^{-}<0 \text { and } a_{i}^{+}>0\right\}\\
    \operatorname{dim} \operatorname{Ker} F^{\star} 
    &=\#\left\{i \in\{1,2\} \suchthat ~ a_{i}^{+}<0 \text { and } a_{i}^{-}>0\right\}
    .\end{align*}


Remark: Resembles formula for computing index in Morse case, number of eigenvalues that change sign.

Remark: Proof will proceed by explicitly computing kernel.

## Proof

Step 1: Transform to Cauchy-Riemann Equations

- Write $a(s) = a_1(s) = a_2(s)$.
- Start with equation on $\RR^2$, $$Y(s, t) = \qty{ Y_1(s, t), Y_2(s, t) }$$
- Replace with equation on $\CC$: $$Y(s, y) = Y_1(s, t) + i Y_2(s, t)$$.
- Rewrite the PDE $F(Y) = 0$ as $\bar \del Y + S(s) Y = 0$, i.e.
\begin{align*}
\frac{\partial}{\partial s}\left(\begin{array}{l}
Y_{1} \\
Y_{2}
\end{array}\right)+\left(\begin{array}{cc}
0 & -1 \\
1 & 0
\end{array}\right) \frac{\partial}{\partial t}\left(\begin{array}{l}
Y_{1} \\
Y_{2}
\end{array}\right)+\left(\begin{array}{cc}
a(s) & 0 \\
0 & a(s)
\end{array}\right)\left(\begin{array}{l}
Y_{1} \\
Y_{2}
\end{array}\right)=0
.\end{align*}

- Change of variables: let $Y  = B\tilde Y$ where $B \in \GL(1, \CC)$ satisfies $\qty{\bar\del + S}B = 0$ to obtain $\bar \del \tilde Y = 0$.

  - Can choose $B = \begin{bmatrix}
  b(s) ) 0 \\
  0 & b(s)
  \end{bmatrix}$ where $\dd{b}{s} = -a(s)b(s)$.
  - Explicitly, we can take the integral 
    $$b(s) = e^{\int_0^s -a(t) ~dt} = e^{-A(s)}$$
