# Fall 2017

## 1

Note that $f(x) = e^x$ is entire and thus equal to its power series.
So $f(x) = \sum_{j=0}^\infty \frac 1 {j!}x^j$.

Letting $f_N(x) = \sum_{j=1}^N \frac 1 {j!} x^j$, we have $f_N(x) \to f(x)$ pointwise on $(-\infty ,\infty)$.

For any compact interval $[-M, M]$, we have

\begin{align*}
\norm{f_N(x) - f(x)}_\infty
&= \sup_{-M\leq x \leq M} ~\abs{\sum_{j=N+1}^\infty \frac 1 {j!} x^j} \\
&\leq \sup_{-M\leq x \leq M} ~ \sum_{j=N+1}^\infty \frac 1 {j!} \abs{x}^j \\
&\leq \sum_{j=N+1}^\infty \frac 1 {j!} M^j \\
&\leq \sum_{j=0}^\infty \frac 1 {j!} M^j \\
&= e^M \\
&<\infty
,\end{align*}

so $f_N \to f$ uniformly on $[-M, M]$ by the M-test.
Thus it converges on any bounded interval.

It does not converge on $\RR$, since $x^N$ is unbounded.

## 2

### a

It suffices to consider the bounded case, i.e. $E \subseteq B_M(0)$ for some $M$.
Then write $E_n = B_n(0) \intersect E$ and apply the theorem to $E_n$, and by subadditivity, $m^*(E) = m^*(\union_n E_n) \leq \sum_n m^*(E_n) = 0$.

**Lemma:** 
$f(x) = x^2, f\inv(x) = \sqrt{x}$ are Lipschitz on any compact subset of $[0, \infty)$.
 
*Proof:*
Let $g = f$ or $f\inv$. 
Then $g\in C^1([0, M])$ for any $M$, so $g$ is differentiable and $g'$ is continuous.
Since $g'$ is continuous on a compact interval, it is bounded, so $\abs{g'(x)} \leq L$ for all $x$.
Applying the MVT,
\begin{align*}
\abs{f(x) - f(y)} = f'(c) \abs{x-y} \leq L \abs{x-y}
.\end{align*}
  
**Lemma:** 
If $g$ is Lipschitz on $\RR^n$, then $m(E) = 0 \implies m(g(E)) = 0$.

*Proof:*
If $g$ is Lipschitz, then 
$$
g(B_r(x)) \subseteq B_{Lr}(x)
,$$ 
which is a dilated ball/cube, and so 
$$
m^*(B_{Lr}(x)) \leq L^n \cdot m^*(B_{r}(x))
.$$

Now choose $\theset{Q_j} \rightrightarrows E$; then $\theset{g(Q_j)} \rightrightarrows g(E)$.

By the above observation,
\begin{align*}
\abs{g(Q_j)} \leq L^n \abs{Q_j}
,\end{align*}

and so 
\begin{align*}
m^*(g(E)) \leq \sum_j \abs{g(Q_j)} \leq \sum_j L^n \abs{Q_j} = L^n \sum_j \abs{Q_j} \to 0 
.\end{align*}

Now just take $g(x) = x^2$ for one direction, and $g(x) = f\inv(x) = \sqrt{x}$ for the other.
$\qed$

### b

> Lemma: $E$ is measurable iff $E = K \disjoint N$ for some $K$ compact, $N$ null.

Write $E = K \disjoint N$ where $K$ is compact and $N$ is null.

Then $\phi\inv(E) = \phi\inv(K \disjoint N) = \phi\inv(K) \disjoint \phi\inv(N)$.

Since $\phi\inv(N)$ is null by part (a) and $\phi\inv(K)$ is the preimage of a compact set under a continuous map and thus compact, $\phi\inv(E) = K' \disjoint N'$ where $K'$ is compact and $N'$ is null, so $\phi\inv(E)$ is measurable.

So $\phi$ is a measurable function, and thus yields a well-defined map $\mathcal L(\RR) \to \mathcal L(\RR)$ since it preserves measurable sets.
Restricting to $[0, \infty)$, $f$ is bijection, and thus so is $\phi$.

$\qed$

## 3

> From homework: $E$ is Lebesgue measurable iff there exists a finite union of closed cubes $A$ such that $m(E\Delta A) < \varepsilon$.

It suffices to show that $S$ is dense in simple functions, and since simple functions are *finite* linear combinations of characteristic functions, it suffices to show this for $\chi_A$ for $A$ a measurable set.

Let $s = \chi_{A}$.
By regularity of the Lebesgue measure, choose an open set $O \supseteq A$ such that $m(O\setminus A) < \varepsilon$.

$O$ is an open subset of $\RR$, and thus $O = \disjoint_{j\in \NN} I_j$ is a disjoint union of countably many open intervals.

Now choose $N$ large enough such that $m(O \Delta I_{N, n}) < \varepsilon = \frac 1 n$ where we define $I_{N, n} \definedas \disjoint_{j=1}^N I_j$.

Now define $f_n = \chi_{I_{N, n}}$, then
\begin{align*}
\norm{s - f_n}_1 = \int \abs{\chi_A - \chi_{I_{N, n}}} = m(A \Delta I_{N, n}) \converges{n\to\infty}\longrightarrow 0
.\end{align*}

Since any simple function is a finite linear combination of $\chi_{A_i}$, we can do this for each $i$ to extend this result to all simple functions.
But simple functions are dense in $L^1$, so $S$ is dense in $L^1$.

## 4

### a

Let $G(x) = \sum_{n=1}^\infty nx(1-x)^n$. 
Applying the ratio test, we have
\begin{align*}
\abs{\frac{(n+1)x(1-x)^{n+1}}{nx(1-x)^n}} = \frac{n+1}{n} \abs{1-x} \converges{n\to\infty}\to \abs{1-x} < 1 \iff 0 \leq x \leq 2
,\end{align*}

and in particular, this series converges on $[0, 2]$. 
Thus its terms go to zero, and $nx(1-x)^n \to 0$ on $[0, 1] \subset [0, 2]$.

To see that the convergence is not uniform, let $x_n = \frac 1 n$ and $\varepsilon > \frac 1 e$, then
\begin{align*}
\sup_{x\in [0, 1]}\abs{nx(1-x)^n - 0} 
\geq \abs{nx_n (1-x_n)^n} 
= \abs{\left( 1 - \frac 1 n\right)^n} 
\converges{n\to\infty}\to e\inv
> \varepsilon
.\end{align*}


### b

> Note: could use the first part with $\sin(x) \leq x$, but then integral ends up more complicated.

Noting that $\sin(x) \leq 1$, we have
We have
\begin{align*}
\abs{\int_0^1  n(1-x)^{n} \sin(x)} 
&\leq \int_0^1  \abs{n(1-x)^n \sin(x)} \\
&\leq \int_0^1  \abs{n (1-x)^n}  \\
&= n\int_0^1 (1-x)^n \\
&= -\frac{n(1-x)^{n+1}}{n+1} \\
&\converges{n\to\infty}\longrightarrow 0
.\end{align*}

## 5


### a

**Lemma:** 
$\dd{}{x} (f \ast \phi) = f \ast (\dd{}{x} \phi)$

*Proof:*

Define
\begin{align*}
D_h \phi(x) \definedas \frac 1 h (\phi(x+h) - \phi(x))
.\end{align*}

Then $D_h\phi \converges{h\to 0}\longrightarrow \dd{}{x}\phi$ pointwise by definition.
It also converges uniformly.

\begin{align*}
\abs{
	(\phi \ast f)_x - \phi_x \ast f
} 
&= \abs{
	\frac {(\phi \ast f)(x+h) - (\phi\ast f)(x)} h - \phi_x \ast f
} \\
&= \abs{\int \left[ \frac{
	\phi(x+h-y) - \phi(x-y)
}{
h
} - \phi_x(x-y) \right]  
f(y) ~dy} \\
&= \abs{\int \left[ D_h \phi(x-y) - \phi_x(x-y) \right] f(y) ~dy} \\
&= ((D_h\phi - \phi_x)\ast f)(x) \\
&\leq 
.\end{align*}
