---
typora-copy-images-to: ./
---

# Mayer Vietoris Problems

# $\RP^2$
We start with a few known facts. Let $A=M$, the Mobius strip, and $B= D^2$, the solid disk.

- $\RP^2 = M \disjoint_\del D^2$
- $H_*(M) = H_*(S^1)$, by a deformation retract of $M$ onto its center circle.
- $H_*(D^2) = \ZZ\delta_0$
- $H_*(S^1)= \ZZ(\delta_0 + \delta_1)$
- $M \intersect D^2 = \del M = S^1$

From Mayer-Vietoris, we have

```latex {cmd:true, hide:false, run_on_save:true}
\documentclass[crop, tikz]{standalone}
\usepackage{tikz}
\usepackage{dsfont}
\usepackage{amsmath, amsthm, amssymb}
\usetikzlibrary{matrix, cd}
\begin{document}

\begin{tikzcd}
 &  &  &  & \cdots 0 \arrow[lllldd, out=0, in=-180, "\delta_3"'] \\
 &  &  &  &  \\
H_2 \partial M \arrow[rr] \arrow[rr, "{(i^*, -j^*)_2}"] &  & H_2 M \oplus H_2 D^2 \arrow[rr, "(l^* - r^*)_2"] &  & H_2 \mathbb{RP}^2 \arrow[lllldd, "\delta_2"', out=0, in=-180] \\
 &  &  &  &  \\
H_1\partial M \arrow[rr, "{(i^*, -j^*)_1}"] &  & H_1 M \oplus H_1 D^2 \arrow[rr, "(l^*-r^*)_1"] &  & H_1 \mathbb{RP}^2 \arrow[lllldd, "\delta_1"', out=0, in=-180] \\
 &  &  &  &  \\
H_0 \partial M \arrow[rr, "{(i^*, -j^*)_0}"] &  & H_0 M \oplus H_0 D^2 \arrow[rr, "(l^* - r^*)_0"] &  & H_0 \mathbb{RP}^2 \arrow[lllldd, "\delta_0"', out=0, in=-180] \\
 &  &  &  &  \\
0 &  &  &  &
\end{tikzcd}

\end{document}
```

and plugging in what is known yields

```latex {cmd:true, hide:false, run_on_save:true}
\documentclass[crop, tikz]{standalone}
\usepackage{tikz}
\usepackage{dsfont}
\usepackage{amsmath, amsthm, amssymb}
\usetikzlibrary{matrix, cd}
\begin{document}

\begin{tikzcd}
 &  &  &  & 0 \arrow[lllldd, out=0, in=-180, "\delta_3"'] \\
 &  &  &  &  \\
0 \arrow[rr] \arrow[rr, "{(i^2, -j^2)}"] &  & 0 \oplus 0 \arrow[rr, "l^2 - r^2"] &  & H_2 \mathbb{RP}^2 \arrow[lllldd, "\delta_2"', out=0, in=-180] \\
 &  &  &  &  \\
\mathbb{Z} \arrow[rr, "{(i^1, -j^1)}"] &  & \mathbb{Z} \oplus 0 \arrow[rr, "l^1-r^1"] &  & H_1 \mathbb{RP}^2 \arrow[lllldd, "\delta_1"', out=0, in=-180] \\
 &  &  &  &  \\
\mathbb{Z} \arrow[rr, "{(i^0, -j^0)}"] &  & \mathbb{Z} \oplus \mathbb{Z} \arrow[rr, "l^0 - r^0"] &  & H_0 \mathbb{RP}^2 \arrow[lllldd, "\delta_0"', out=0, in=-180] \\
 &  &  &  &  \\
0 &  &  &  &
\end{tikzcd}

\end{document}
```

where $i: S^1 \into M$ and $j: S^1 \into D^2$.

We can then identify all of the induced maps:

- $i^2: H_2 \del M \into H_2 M \implies i^2: 0 \to 0 \implies i^2 = 0$
- $i^1: H_1 \del M \into H_1 M$, i.e. $i^1: \ZZ \to \ZZ$ where $1 \mapsto 2$
  - Since $M$ deformation retracts onto its center circle, $H_1 M \cong H_1 S_M$ where $S_M$ is the center circle (homotopies induce isomorphisms on homology). But $H_1 \del M$ is generated by a cycle of edges with includes into $\del M$, which retracts onto a cycle that double covers $S_M$, so this map acts by doubling the generator.
- $i^0: H_0 \del M \into H_0 M$, i.e. $i^0: \ZZ \to \ZZ$
- $j^2: H_2 \del M \to H_2 D^2 \implies j^2: 0 \to 0 \implies j^2 = 0$
- $j^1: H_1 \del M \to H_1 D^2 \implies j^1: \ZZ \to 0 \implies j^1 = 0$
- $j^0: H_0 \del M \to H_0 D^2 \implies j_0: \ZZ \to \ZZ$

So we can that the only nontrivial maps are $j^0, i^0, i^1$.



## Claim: $H_2(\RP^2) = 0$:

We consider the portion of the sequence $$\cdots 0 \mapsvia{} H_2{\RP^2} \mapsvia{\delta_2} H_1 \del M \mapsvia{(i^1, -j^1)} H_1M \oplus H_1 D^2 \cdots\\
\cdots 0 \mapsvia{} H_2\RP^2 \mapsvia{\delta_2} \ZZ \mapsvia{(i^1, -j^1)} \ZZ \oplus 0 \cdots$$

We will show that $\ker \delta_2 = \im \delta_2 = 0$. By the first isomorphism theorem, we would then have $\frac{H_2 \RP^2}{\ker \delta_2} \cong \im \delta_2$ yielding $\frac{H_2 \RP^2}{0} = H_2 \RP^2 \cong 0$.

- *Claim: $\ker \delta_2 = 0$*

  This follows because it is on the left tail of an exact sequence, where $\ker \delta_2 = \im 0 = 0$.

- *Claim: $\im \delta_2 = 0$*

  $$(i^1, -j^1): H_1 \del M \to H_1 M \oplus H_1 D^2$$ is injective; explicitly, it is the map $$M_2: \ZZ \to \ZZ \oplus 0\\~1\mapsto (2, 0)$$

  From above, know that $-j^1$ is a zero map, and that $i^1$ doubles each generator. By this explicit construction, it is injective since 0 maps to 0.

  But then $\ker (i^1, -j^1) = \im \delta_2 = 0$ by exactness.

So now we have:
```latex {cmd:true, hide:false, run_on_save:true}
\documentclass[crop, tikz]{standalone}
\usepackage{tikz}
\usepackage{dsfont}
\usepackage{amsmath, amsthm, amssymb}
\usetikzlibrary{matrix, cd}
\begin{document}

\begin{tikzcd}
 &  &  &  & 0 \arrow[lllldd, out=0, in=-180, "0"'] \\
 &  &  &  &  \\
0 \arrow[rr] \arrow[rr, "{0\times 0}"] &  & 0 \oplus 0 \arrow[rr, "0"] &  & 0 \arrow[lllldd, "0"', out=0, in=-180] \\
 &  &  &  &  \\
\mathbb{Z} \arrow[rr, "{x \mapsto (2x, 0)}"] &  & \mathbb{Z} \oplus 0 \arrow[rr, "l^1-r^1"] &  & H_1 \mathbb{RP}^2 \arrow[lllldd, "\delta_1"', out=0, in=-180] \\
 &  &  &  &  \\
\mathbb{Z} \arrow[rr, "{(i^0, -j^0)}"] &  & \mathbb{Z} \oplus \mathbb{Z} \arrow[rr, "l^0 - r^0"] &  & H_0 \mathbb{RP}^2 \arrow[lllldd, "\delta_0"', out=0, in=-180] \\
 &  &  &  &  \\
0 &  &  &  &
\end{tikzcd}

\end{document}
```

## Claim: $H_1(\RP^2) = \ZZ_2$

Here we are examining this portion of the sequence:

$$
\cdots \ZZ \mapsvia{x\mapsto (2x, 0)} H_1 M \oplus H_1 D^2 \mapsvia{l^1 - r^1} H_1 \RP^1 \mapsvia{\delta_1} H_0 \del M \mapsvia{(i^0, -j^0)} H_0 M \oplus H_0 D^2 \cdots\\
\cdots \ZZ \mapsvia{x\mapsto (2x, 0)} \ZZ \oplus 0 \mapsvia{l^1-r^1} H_1 \RP^1 \mapsvia{\delta_1} \ZZ \mapsvia{(i^0, -j^0)} \ZZ \oplus \ZZ\cdots
$$

In general, we have the first isomorphism theorem: given any map $f$ we have $\frac{\mathrm{dom}f}{\ker f} \cong \im f$. Here we will take $f = l^1 - r^1$ and identify the necessary components to apply this theorem.

- Claim: $\im l^1 - r^1 = H_1 \RP^2$.
  - We use the fact that the maps $(i^*, j^*)$ are all injections, so in particular $0 = \ker (i^0, j^0) = \im \delta_1$ by exactness. Consequently $\ker \delta_1 = H_1\RP^1 = \im l^1 - r^1$ by exactness.
- What is $\ker (l^1-r^1)$?
  - By exactness, $\ker (l^1 - r^1) = \im (x \mapsto (2x, 0)) = 2\ZZ \oplus 0$

By the first isomorphism theorem, we have $\im (l^1-r^1) \cong \frac{\mathrm{dom} (l^1-r^1)}{\ker (l^1-r^1)} = \frac{\ZZ\oplus 0}{2\ZZ \oplus 0} \cong \ZZ_2$.

Note that $l^1 - r^1$ is a nontrivial homomorphism from $2\ZZ\cong \ZZ$ to $\ZZ_2$, of which there is only one: the natural quotient map $x \mapsto x \mod 2$.

There is also no nontrivial homomorphism from $\ZZ_2 \to \ZZ$, so $\delta_1 = 0$.

We now have:
```latex {cmd:true, hide:false, run_on_save:true}
\documentclass[crop, tikz]{standalone}
\usepackage{tikz}
\usepackage{dsfont}
\usepackage{amsmath, amsthm, amssymb}
\usetikzlibrary{matrix, cd}
\begin{document}

\begin{tikzcd}
 &  &  &  & 0 \arrow[lllldd, out=0, in=-180, "0"'] \\
 &  &  &  &  \\
0 \arrow[rr] \arrow[rr, "{0\times 0}"] &  & 0 \oplus 0 \arrow[rr, "0"] &  & 0 \arrow[lllldd, "0"', out=0, in=-180] \\
 &  &  &  &  \\
\mathbb{Z} \arrow[rr, "{x \mapsto (2x, 0)}"] &  & \mathbb{Z} \oplus 0 \arrow[rr, "x \mapsto x \mod 2"] &  & \mathbb{Z}_2 \arrow[lllldd, "0"', out=0, in=-180] \\
 &  &  &  &  \\
\mathbb{Z} \arrow[rr, "{(i^0, -j^0)}"] &  & \mathbb{Z} \oplus \mathbb{Z} \arrow[rr, "l^0 - r^0"] &  & H_0 \mathbb{RP}^2 \arrow[lllldd, "\delta_0"', out=0, in=-180] \\
 &  &  &  &  \\
0 &  &  &  &
\end{tikzcd}

\end{document}
```

## Claim: $H_0(\RP^2) = \ZZ$

Here we examine


$$
H_1\RP^2 \mapsvia{\delta_1} H_0 \del M \mapsvia{(i^0, j^0)} H_0 M \oplus H_0 D^2 \mapsvia{l^0 - r^0} H_0\RP^2 \mapsvia{\delta_0} 0\\
\ZZ_2 \mapsvia{\delta_1} \ZZ \mapsvia{(i^0, j^0)} \ZZ \oplus \ZZ \mapsvia{l^0 + r^0} H_0\RP^2 \mapsvia{\delta_0} 0
$$

Since there is no nontrivial homomorphism from $\ZZ_2 \to \ZZ$, we have $\delta_1 = 0$.

We also have $\delta_0 = 0$ and $\ker \delta_0 = H_0 \RP^2 = \im l^0 + r^0$ making $l^0 + r^0$ surjective, so by the first isomorphism theorem we have $H_0 \RP^2 \cong \frac{\ZZ \oplus \ZZ}{\ker l^0 + r^0} = \frac{\ZZ \oplus \ZZ}{\im (i^0, j^0)}$

By a similar argument used earlier, the double covering of the boundary circle $\del M$ over $S^1$ yields the map $(i^0, j^0): \ZZ \into \ZZ \oplus \ZZ$ given by $x \mapsto (2x, 2x)$ with

## Summary

With all of this information, we finally have

```latex {cmd:true, hide:false, run_on_save:true}
\documentclass[crop, tikz]{standalone}
\usepackage{tikz}
\usepackage{dsfont}
\usepackage{amsmath, amsthm, amssymb}
\usetikzlibrary{matrix, cd}
\begin{document}

\begin{tikzcd}
 &  &  &  & 0 \arrow[lllldd, out=0, in=-180, "0"'] \\
 &  &  &  &  \\
0 \arrow[rr] \arrow[rr, "{0 \mapsto (0,0)}"] &  & 0 \oplus 0 \arrow[rr, "{(0,0)  \mapsto 0}"] &  & 0 \arrow[lllldd, "0"', out=0, in=-180] \\
 &  &  &  &  \\
\mathbb{Z} \arrow[rr, "{x\mapsto (2x, 0)}"] &  & 2\mathbb{Z} \oplus 0 \arrow[rr, "{(x,0) \mapsto x \mod 2}"] &  & \mathbb{Z}_2 \arrow[lllldd, "0"', out=0, in=-180] \\
 &  &  &  &  \\
\mathbb{Z} \arrow[rr, "{x \mapsto (2x, x)}"] &  & 2\mathbb{Z} \oplus \mathbb{Z} \arrow[rr, "{(x,y) \mapsto x-y}"] &  & \mathbb{Z} \arrow[lllldd, "0"', out=0, in=-180] \\
 &  &  &  &  \\
0 &  &  &  &
\end{tikzcd}

\end{document}
```

And so we find $H_*(\RP^2) = \ZZ \delta_0 + \ZZ_2\delta_1$

# Cellular Homology

# Degree

# UCT

# Homological Algebra
