# Friday, September 25

## Review and Proposition

From last time: Steinberg's tensor product.

Let $G$ be a reductive algebraic group scheme over $k$ with $\ch(k) > 0$.
We have a Frobenius $F:G\to G$, we iterate to obtain $F^r$ and examine the Frobenius kernels $G_r\da \ker F^r$.

If we have a representation $\rho: G\to \GL(M)$, we can "twist" by $F^r$ to obtain $\rho^{(r)}: G \to \GL(M^{(r)})$.
We have

<!--\begin{center}-->
<!--\begin{tikzcd}-->
<!--G \ar[r, "{F^r}"] \ar[rr, "{\rho^{(r)}}" & G\ar[r, "\rho"] & \GL(M)-->
<!--\end{tikzcd}-->
<!--\end{center}-->

Here $M^{(r)}$ has the same underlying vector space as $M$, but a new module structure coming from $\rho^{(r)}$.
Note that $G_r$ acts trivially on $M^{(r)}$.

- $\ts{L(\lambda) \st \lambda \in X(T)_+}$ are the simple $G\dash$modules,
- $\ts{L_r(\lambda) \st \lambda \in X_r(T)_+}$ are the simple $G_r\dash$modules,

Note that $L(\lambda)\downarrow_{G_r}$ is semisimple, equal to $L_r(\lambda)$ for $\lambda \in X_r(T)$.

> 1960's, Curtis and Steinberg.

:::{.proposition title="?"}
Let $\lambda \in X_r(T)$ and $\mu \in X(T)_+$.
Then
\[  
L(\lambda + p^r \mu) \cong L(\lambda) \tensor L(\mu)^{(r)}
.\]

:::

Recall that socle formula: letting $M$ be a $G\dash$module, we have an isomorphism of $G\dash$modules:
\[ 
\soc_{G_r} \cong \bigoplus_{\lambda \in X_r(T)} L(\lambda) \tensor \hom_{G_r}(L(\lambda), M)
.\]


## Proof

Let $M = L(\lambda + p^r \mu)$.
Then from the socle formula, only one summand is nonzero, and thus $\hom_{G_r}(L(\lambda), M)$ must be simple.
Then there exists a $\tilde \lambda \in X_r(T)$ and a $\tilde \mu \in X(T)_+$ such that
\[  
M = L(\tilde \lambda) \tensor L(\tilde\mu)^{(r)}
.\]

We now compare highest weights: 
\[  
\lambda + p^r \mu = \tilde \lambda + p^r \tilde \mu \implies \lambda = \tilde \lambda \qtext{and} \mu = \tilde \mu
.\]

:::{.theorem title="Steinberg"}
Let $\lambda \in X(T)_+$, with a $p\dash$adic expansion
\[  
\lambda = \lambda_0 + \lambda_1 p + \cdots + \lambda_m p^m
.\]
where $\lambda_j \in X_q(T)$ for all $j$.
Then
\[  
L(\lambda) = L(\lambda_0) \bigotimes_{j=1^m} L(\lambda_j)^{(j)}
.\]
:::
