# Fall 2018

## 1

### a

We know that every $p\dash$subgroup is contained in some Sylow $p\dash$subgroup, so $P \subseteq S_p^i$ for some $S_p^i \in \mathrm{Syl}_p(G)$.

Since $P$ is normal in $G$, we have $gPg\inv = P$ for all $g\in G$.

If $S_p^j$ is any other Sylow $p\dash$subgroup, we have $gS_p^i g\inv = S_p^j$ for some $g\in G$.

But then $P = gPg\inv \subseteq gS_p^i g\inv = S_p^j$.

### b

?

TODO

## 2

### a

> - $G_a = \mathrm{Stab}_G(a) = \theset{g\in G \suchthat g\actson a = a}$
> - $G_b = \mathrm{Stab}_G(b) = \theset{g\in G \suchthat g\actson b = b}$
> - $G\cdot x = \mathcal O_x = \theset{g\actson x \suchthat g\in G}$

Suppose $a,b \in X$ where $a \in G\cdot b$, so they belong to the same orbit.
Then $a = h\actson b$ for some $h\in G$.

Then
\begin{align*}
g\in G_a 
\iff g\actson a &= a \\
\iff g \actson (h\actson b) &= h\actson b \\
\iff gh \actson b &= h\actson b \\
\iff h\inv gh \actson b &= b \\
\iff h\inv g h &\in G_b
,\end{align*}

so $g\in G_a \iff hgh\inv \in G_b$ and so the stabilizers of any two elements in the same orbit are conjugate.

### b

Suppose $\abs{H} = n$ and thus $\abs{G} = nm$ for some $m = [G: H] \geq 2$ by Lagrange since $H$ is proper.

Let $G$ act on its subgroups by conjugation, 

- The orbit $G\cdot H$ is the set of all conjugate subgroups, and

- The stabilizer of $H$ is $G_H = N_G(H)$.

By orbit-stabilizer,
\begin{align*}
G\cdot H = [G: G_H] = [G: N_G(H)]
.\end{align*}

Let $\abs H = n$, and note that all conjugate subgroups have the same order.

Then
\begin{align*}
H \leq N_G(H) 
&\implies [G: N_G(H)] \leq [G: H] = m
.\end{align*}

and each conjugate contains the identity element, so

\begin{align*}
\union_{g\in G} gHg\inv &
\leq 1 + \sum_{H' \in G\cdot H} \left( \abs{H'} - 1 \right) \\
&= 1 + \sum_{H' \in G\cdot H} n - 1 \\
&= 1 + (n-1) \abs{G\cdot H} \\
&= 1 + (n-1) [G: N_G(H)] \\
&\leq 1 + (n-1) [G: H] \\
&= 1 + (n-1) m\\
&= 1 + nm - m \\
&= 1  + \abs{G} - m \\
&= \abs{G} - (m-1) \\
&\leq \abs{G} - 1 \quad \text{since } m \geq 2\\
&< \abs G
.\end{align*}

> Todo: not an ideal proof. Doesn't use the first part..?

### c

Noting that $G\actson S$ transitively iff there is only one orbit and $\abs {S/G} = 1$, by Burnside's lemma we have
\begin{align*}
1 = \abs{S/G} = \frac{1}{\abs G} \sum_{g\in G} \abs{S^g} \implies \abs{G} = \sum_{g\in G} \abs{S^g}
\end{align*}

where $S^g = \theset{s\in S \suchthat g\actson s = s ~\forall g\in G}$.

We can now note that $S^e = S$ and so $\abs{S^e} \geq 2$, not every other term in the sum can be greater than 1.
So there is some $g$ such that $\abs{S^g} = 0$, so $g$ has no fixed points.

$\qed$

## 3

### a

False: take $L/K/F = \QQ(\zeta_2, \sqrt[3] 2) \to \QQ(\sqrt[3] 2) \to \QQ$.

Then $L/F$ is Galois, since it is the splitting field of $x^3 - 2$ and $\QQ$ has characteristic zero.

But $K/F$ is not Galois, since it is not the splitting field of any irreducible polynomial.

### b



### c