# Wednesday November 20

Last time:

$$
\ZZ \Lambda \iff \theset{ \lieh^* \to \ZZ_{\geq 0} \mid \sim  } \\
e(\mu) \mapsto e_\mu \\
e(\lambda) e(\mu) = e(\lambda + \mu) \mapsto f \star g(\lambda) = \sum_{a+b=\lambda} f(a) g(b)
$$

and $\mathrm{ch} L(\lambda) = \sum_{\mu \in \Lambda} \dim L(\lambda)_\mu e(\mu)$.

We have the Kostant function $p(\lambda) = \# \theset{ (k_\alpha)_\alpha \mid -\lambda = \sum_{\alpha\in\Phi^+} k_\alpha \alpha  }$ 
and the Weyl function $q = e_\rho \star \prod_{\alpha\in\Phi^+}(1 - e_{-\alpha}) = \prod_{\alpha\in\Phi^+} (e_{\alpha/2} - e_{-\alpha/2})$.

Lemma:
$p\star e_\lambda = \mathrm{ch} M(\lambda)$, so $q \star \mathrm{ch} M(\lambda) = e_{\lambda + \rho}$ and $q \star p = e_\rho$.

## Weyl's Character Formula  (24.2-3)

Definition: 
The *dot action* of $W$ is given by $w\cdot \lambda = w(\lambda + \rho) - \rho$, i.e. a reflection for hyperplanes passing through $-\rho$.

E.g. for type $A2$, where $W(0) = 0$, we have:

![Type A2](figures/2019-11-20-09:19.png)

And for the dot action, we have

![Image](figures/2019-11-20-09:22.png)

where $W \cdot 0 = 0$ and $s(\alpha_1) = -\alpha_1$.

**Theorem (Harish-Chandra):**
If $L(\mu)$ is a composition factor of $M(\lambda)$, then $\mu \in W\cdot \lambda$ for $\mu \leq \lambda$.

Proof:
Postponed.

> $\mathrm{ch}$ are characters, $L(\lambda)$ is a Verma module.

Remark: if we sum over $\mu \leq \lambda$, we obtain

\begin{align*}
\mathrm{ch} M(\lambda) &= \sum_{\mu \in W \cdot \lambda} a_{\lambda \mu} \mathrm{ch} L(\mu) \\
\mathrm{ch} L(\lambda) &= \sum_{\mu \in W \cdot \lambda} b_{\lambda \mu} \mathrm{ch} M(\mu) 
&= \sum_{W\cdot \lambda \in \Lambda} c_{\lambda W} \mathrm{ch} M(w\cdot \lambda)
.\end{align*}

**Theorem (Weyl's Character Formula):**
If $\lambda \in \Lambda^+$, then 
$$
\mathrm{ch} L(\lambda) = \frac{
\sum_{w\in W} (-1)^{\ell(w)} e(w \cdot \lambda)
}{
\sum_{w\in W} (-1)^{\ell(w)} e(w\cdot 0)
}
$$

*Proof*:

We have $\mathrm{ch} L(\lambda) = \sum_{w} c_{\lambda w} \mathrm{ch} M(w\cdot \lambda)$, and so by the lemma, 
$$
q \ast \mathrm{ch} L(\lambda) = \sum c_{\lambda w} q \star \mathrm{ch} M(W(\lambda + \rho) - \rho)$ = \sum_w c_{\lambda w} e_{W(\lambda + p)}
$$

Thus for all $\alpha \in \Phi^+$, we have
$$
s_\alpha(q \star \mathrm{ch} L(\lambda)) = \sum_w c_{\lambda, s_\alpha w} e_{w(\lambda + \rho)}
$$

On the other hand, by part (c) of the lemma, we have 
$$
(s_\alpha \star \q) \star \mathrm{ch} L(\lambda) = -q \star \mathrm{ch} L(\lambda) = \sum_w -c_{\lambda, w} e_{w(\lambda+\rho)}$
$$

which implies that $c_{\lambda, s_\alpha w} = -c_{\lambda, w}$ by comparing term-by-term, and thus $c_{\lambda, w} = (-1)^{\ell(w)}$ because $c_{\lambda e} = 1$.

