---
title: "Algebra"
---

---

# Lecture 1 (Thu 15 Aug 2019)

Definition: A *group* is an ordered pair $(G, \wait: G\cross G \to G)$ where $G$ is a set and $\wait$ is a binary operation, which satisfies the following axioms:

1. Associativity: $(g_1 g_2)g_3 = g_1(g_2 g_3)$
2. Identity: $\exists e\in G \suchthat  ge = eg = g$
3. Inverses: $g\in G \implies \exists h\in G \suchthat gh = gh = e$.

Some examples of groups:

- $(\ZZ, +)$
- $(\QQ, +)$
- $(\QQ\units, \times)$
- $(\RR\units, \times)$
- ($\GL(n, \RR), \times) = \theset{A \in \mathrm{Mat}_n \suchthat \det(A) \neq 0}$
- $(S_n, \circ)$

Definition: A subset $S \subseteq G$ is a *subgroup* of $G$ iff

1. $s_1, s_2 \in S \implies s_1 s_2 \in S$
2. $e\in S$
3. $s\in S \implies s\inv \in S$

We denote such a subgroup $S \leq G$.

Examples:

- $(\ZZ, +) \leq (\QQ, +)$
- $\SL(n, \RR) \leq \GL(n, \RR)$, where $\SL(n, \RR) = \theset{A\in \GL(n, \RR) \suchthat \det(A) = 1}$

Definition: A group $G$ is cyclic iff $G$ is generated by a single element.

Exercise: Show $\generators{g} = \theset{g^n \suchthat n\in\ZZ} \cong \intersect \theset{H \leq G \suchthat g \in H}$.

Theorem: Let $G$ be a cyclic group, so $G \generators{g}$.

1. If $\abs{G} = \infty$, then $G \cong \ZZ$.
2. If $\abs{G} = n < \infty$, then $G \cong \ZZ_n$


Definition: Let $H \leq G$, and define a *right coset of $G$* by $aH = \theset{ah \suchthat H \in H}$. A similar definition can be made for *left cosets*.

Then $aH = bH \iff b\inv a \in G$ and $Ha = Hb \iff ab\inv \in H$.

Some facts:

- Cosets partition $H$, i.e. $b\not\in H \implies aH \intersect bH = \theset{e}$.
- $\abs{H} = \abs{aH} = \abs{Ha}$ for all $a\in G$.

Theorem (Lagrange): If $G$ is a finite group and $H \leq G$, then $\abs{H} \divides \abs{G}$.

Definition: $N \leq G$ is *normal* iff $gN = Ng$ for all $g\in G$, or equivalently $gNg\inv \subseteq N$. I denote this $N \normal G$.

When $N \normal G$, the set of left/right cosets of $N$ themselves have a group structure. So we define $G/N = \theset{gN \suchthat g\in G}$ where $(g_1 N)(g_2 N) = (g_1 g_2) N$.
