# Wednesday, March 24


:::{.remark}
Last time: we're trying to prove the classical convergence theorem in the bounded case.
We have 
\[
E_{pq}^1 = H_{p+q}( F_p C/ F_{p-1} C ) \abuts H_{p+q}C
.\]
We'd like this converge, i.e. the $E^\infty$ page will be the sections of $H_{p+q}C$.
Writing $C_n'\da F_p C_n$ for the filtered pieces, we have

\begin{tikzcd}
	{C_n'} && {C_n} \\
	{Z_n'} && {Z_n} \\
	{B_n'} && {B_n}
	\arrow[hook, from=3-1, to=3-3]
	\arrow[hook, from=2-1, to=2-3]
	\arrow[hook, from=1-1, to=1-3]
	\arrow[hook, from=1-3, to=2-3]
	\arrow[hook, from=2-3, to=3-3]
	\arrow[hook, from=1-1, to=2-1]
	\arrow[hook, from=2-1, to=3-1]
\end{tikzcd}

> [Link to Diagram](https://q.uiver.app/?q=WzAsNixbMCwwLCJDX24nIl0sWzIsMCwiQ19uIl0sWzAsMSwiWl9uJyJdLFsyLDEsIlpfbiJdLFswLDIsIkJfbiciXSxbMiwyLCJCX24iXSxbNCw1LCIiLDAseyJzdHlsZSI6eyJ0YWlsIjp7Im5hbWUiOiJob29rIiwic2lkZSI6InRvcCJ9fX1dLFsyLDMsIiIsMCx7InN0eWxlIjp7InRhaWwiOnsibmFtZSI6Imhvb2siLCJzaWRlIjoidG9wIn19fV0sWzAsMSwiIiwwLHsic3R5bGUiOnsidGFpbCI6eyJuYW1lIjoiaG9vayIsInNpZGUiOiJ0b3AifX19XSxbMSwzLCIiLDEseyJzdHlsZSI6eyJ0YWlsIjp7Im5hbWUiOiJob29rIiwic2lkZSI6InRvcCJ9fX1dLFszLDUsIiIsMSx7InN0eWxlIjp7InRhaWwiOnsibmFtZSI6Imhvb2siLCJzaWRlIjoidG9wIn19fV0sWzAsMiwiIiwxLHsic3R5bGUiOnsidGFpbCI6eyJuYW1lIjoiaG9vayIsInNpZGUiOiJ0b3AifX19XSxbMiw0LCIiLDEseyJzdHlsZSI6eyJ0YWlsIjp7Im5hbWUiOiJob29rIiwic2lkZSI6InRvcCJ9fX1dXQ==)

Then the induced filtration on homology is 
\[
H_n' \da {Z_n' \over B_n'} &\injects H_n \da {Z_n\over B_n} \\
z' + B_n' &\mapsto z' + B_n
.\]

:::


:::{.proof title="of classical convergence theorem"}
As discussed, we have a natural bounded filtration on each $H_n C$.
Fixing $p, n$
and writing $q = n-p$, we have
\[
A_p^r = \ts{ c \in F_p C_n \st d(c) \in F_{p-r} C_{n-1} } 
.\]
This stabilizes for large $r$, namely whenever $F_{p-r} C_{n-1} = 0$ (which happens since the complex is bounded).
Call the stabilized object $A_p^{\infty } \da \ts{ c\in F_p C_n \st d(c) = 0 }$, which is $\ker d$ in the $p$th filtered piece.
Some facts:

0. $Z_p^r = \eta_p(A_p^r$ where
\[
\eta_p: F_p C_n \to {F_p C_n \over F_{p-1} C_n }
\]
where $Z_p^{\infty } = \eta_p(A_p^{\infty })$.

1. $A_p^{\infty } \da \ker (F_p C_n \mapsvia{d} F_p C_{n-1} )$, which is the "numerator" of $F_p H_n C$.

2. $d(C_{n+1}) \intersect F_p C_n = \union_{r\in \ZZ} d(A_{p+r}^r )$:

\begin{tikzcd}
	&&&& {A_{p+r}} \\
	&&&& {F_{p+r}C_{n+1}} & {C_{n+1}} \\
	{F_p C_n}
	\arrow["d"', from=1-5, to=3-1]
	\arrow[hook, from=1-5, to=2-5]
	\arrow[hook, from=2-5, to=2-6]
\end{tikzcd}

> [Link to Diagram](https://q.uiver.app/?q=WzAsNCxbNCwwLCJBX3twK3J9Il0sWzQsMSwiRl97cCtyfUNfe24rMX0iXSxbNSwxLCJDX3tuKzF9Il0sWzAsMiwiRl9wIENfbiJdLFswLDMsImQiLDJdLFswLDEsIiIsMix7InN0eWxlIjp7InRhaWwiOnsibmFtZSI6Imhvb2siLCJzaWRlIjoidG9wIn19fV0sWzEsMiwiIiwyLHsic3R5bGUiOnsidGFpbCI6eyJuYW1lIjoiaG9vayIsInNpZGUiOiJ0b3AifX19XV0=)

3. Recall that we defined $B_p^r \da \eta_p( d A_{p+r-1}^{r-1} )$.
  We can write \( B_p^{\infty } = \eta_p (\union_r dA_{p+r}^r ) \).


:::


