# My Common Mistakes

\[
-x^{-2} &\neq \int x^{-1} = \int \frac{1}{x} = \ln x \\ 
\frac{1}{x} &\neq \int \ln x = x\ln x - x \\
\int x^{-k} = \frac{1}{-k+1}x^{-k+1} &\neq \frac{1}{-(k+1)}x^{-(k+1)} \\
\text{ e.g. } \int x^{-2} = -x^{-1} &\neq -\frac{1}{3}x^{-3}
\lim_{n\to\infty} \frac{n}{n+1} = 1 \neq 0\\
\frac{\partial}{\partial x}a^x = \frac{\partial}{\partial x}e^{x\ln a} = e^{x\ln a} \ln a = a^x \ln a.
\]

Exponentials: when in doubt, write $a^b = e^{b\ln a}$

\[
\frac{\partial}{\partial x} x^{f(x)} = ?
\]

\[
\sum x^k = \frac{1}{1-x} \neq \frac{1}{1+x} = \sum (-1)^k x^k
\]

---

\[
               &  & \sin              &  & \cos               &  & \tan \\ \hline \\
0              &  & \frac{\sqrt 0}{2} &  & \frac{\sqrt 4}{2}  &  & 0\\ \\
\frac{\pi}{6}  &  & \frac{\sqrt 1}{2} &  & \frac{\sqrt 3}{2}  &  & \frac{1}{\sqrt 3}\\ \\
\frac{\pi}{4}  &  & \frac{\sqrt 2}{2} &  & \frac{\sqrt{2}}{2} &  & 1 \\ \\
\frac{\pi}{3}  &  & \frac{\sqrt 3}{2} &  & \frac{\sqrt 1}{2}  &  & \frac{\sqrt 3}{1}\\ \\
\frac{\pi}{2}  &  & \frac{\sqrt 4}{2} &  & \frac{\sqrt 0}{2}  &  & \infty
\]

\[
(a+b)^2 =                    &  & \hspace{20em} a^2 + b^2 + 2ab \\
(a-b)^2 =                    &  & a^2 + b^2 - 2ab \\
a^2+b^2 =                    &  & (a+b)^2 + 2ab \\
a^2- b^2 =                   &  & (a+b)(a-b) \\
(a+b)^3 =                    &  & a^3 + b^3 + 3(a^2b + ab^2) \\
(a-b)^3 =                    &  & a^3 -b^3 + 3(-a^2b +ab^2) \\
a^3 + b^3 =                  &  & (a+b)(a^2+b^2-ab) \\
a^3 - b^3 =                  &  & (a-b)(a^2+ b^2 + ab) \\
(\sqrt a + \sqrt b)^2 =      &  & a + b + 2\sqrt{ab} \\
(\sqrt a - \sqrt b)^2 =      &  & a + b - 2\sqrt{ab} \\
(a+\sqrt{b})(a-\sqrt{b}) =   &  & a^2 - b \\
(a+i\sqrt{b})(a-i\sqrt{b}) = &  & a^2 + b \\
(a+b)(a-b) =                 &  & a^2 + b^2
\]


\[
\frac{\partial f}{\partial{x}}\Leftarrow &  & f                       &  & \Rightarrow\int f dx   \\
\hline \\
\frac{1}{2\sqrt{x}}                      &  & \sqrt{x}                &  & \frac{2}{3}x^{\frac{3}{2}} \\
nx^{n-1}                                 &  & x^n, n \neq -1          &  & \frac{1}{n+1}x^{n+1} \\
\frac{1}{x}                              &  & {\ln(x)}                &  & x\ln(x) - x \\
a^x\ln(a)                                &  & a^x                     &  & \frac{a^x}{\ln a} \\
\cos(x)                                  &  & \sin(x)                 &  & -\cos(x) \\
-\sin(x)                                 &  & \cos(x)                 &  & \sin(x) \\
2\sec^2(x)\tan(x)                        &  & \sec^2(x)               &  & \tan(x) \\
2\csc^2(x)\cot(x)                        &  & \csc^2(x)               &  & -\cot(x) \\
\sec^2(x)                                &  & \tan(x)                 &  & \ln\abs{\sec(x)} \\
\sec(x)\tan(x)                           &  & \sec(x)                 &  & \ln\abs{\sec(x) + \tan(x)} \\
-\csc(x)\cot(x)                          &  & \csc(x)                 &  & \ln\abs{\csc(x)-\cot(x)} \\
\frac{1}{1+x^2}                          &  & {\tan^{-1}(x)}          &  & x\tan^{-1}x - \frac{1}{2}\ln(1+x^2) \\
\frac{1}{\sqrt{1-x^2}}                   &  & {\sin^{-1}(x)}          &  & x\sin^{-1}x+ \sqrt{1-x^2} \\
-\frac{1}{\sqrt{1-x^2}}                  &  & {\cos^{-1}(x)}          &  & x\cos^{-1}x -\sqrt{1-x^2} \\
\frac{1}{\sqrt{x^2+a}}                   &  & \ln\abs{x+\sqrt{x^2+a}} &  & \cdot\\
-\csc^2(x)                               &  & \cot(x)                 &  & ? \\
?                                        &  & \cos^2(x)               &  & ? \\
?                                        &  & \sin^2(x)               &  & ? \\
?                                        &  & xe^{ax}                 &  & \frac { 1 } { a ^ { 2 } } ( a x - 1 ) e ^ { a x } \\
?                                        &  & e^{ax}\sin(bx)          &  & \frac { 1 } { a ^ { 2 } + b ^ { 2 } } e ^ { a x } ( a \sin b x - b \cos b x ) \\
?                                        &  & e^{ax}\cos(bx)          &  & \frac { 1 } { a ^ { 2 } + b ^ { 2 } } e ^ { a x } ( a \sin b x + b \cos b x ) \\
?                                        &  & ?                       &  & ?
\]



\[
\sqrt{a^2-x^2}   &  & \Rightarrow &  & x = a\sin(\theta)  &  & dx = a\cos(\theta)~d\theta \\
\sqrt{a^2+x^2}   &  & \Rightarrow &  & x = a\tan(\theta)  &  & dx = a\sec^2(\theta)~d\theta \\
\sqrt{x^2 - a^2} &  & \Rightarrow &  & x = a \sec(\theta) &  & dx = a\sec(\theta)\tan(\theta)~d\theta
\]


\[
p(y)y' = q(x)                  &  & \hspace{10em} \text{separable} \\ \\
y'+p(x)y = q(x)                &  & \text{integrating factor} \\ \\
y' = f(x,y), f(tx,ty) = f(x,y) &  & y = xV(x)\text{ COV reduces to separable} \\ \\
y' +p(x)y = q(x)y^n            &  & \text{Bernoulli, divide by $y^n$ and COV $u = y^{1-n}$} \\ \\
M(x,y)dx + N(x,y)dy = 0        &  & M_y = N_x: \phi(x,y) = c (\phi_x =M, \phi_y = N) \\ \\
P(D)y = f(x,y)                 &  & x^ke^{rx} \text{ for each root }
\]
